progress on proving functional correctness for rsapss

specs/experimental/rsapss/Spec.RSA.Bignum.fst
@@ -26,103 +26,174 @@ let mod_inv_u64 n0 =
   vb
 
 (* Montgomery's arithmetic *)
-val mont_reduction_f:
+val mont_pred:
   #nBits:size_pos -> #cBits:size_pos ->
   rBits:size_pos{nBits < rBits /\ nBits+1+rBits < max_size_t} ->
-  nInv_u64:bignum 64 -> n:bignum nBits ->
+  nInv_u64:bignum 64 -> n:bignum nBits{bn_v n > 0} ->
   c:bignum cBits ->
-  i:size_nat{64 * (i+1) <= rBits} -> res:bignum (nBits + 1 + rBits) ->
-  Tot (res:bignum (nBits + 1 + rBits))
-  #reset-options "--z3rlimit 30 --max_fuel 0"
+  i:size_nat{i <= rBits / 64} -> res:bignum (nBits + 1 + rBits) -> Tot Type0
+let mont_pred #nBits #cBits rBits nInv_u64 n c i res = bn_v res % bn_v n = bn_v c % bn_v n && bn_v res <= bn_v c + (pow2 (64*i) - 1) * bn_v n
+
+val mont_reduction_f:
+  #nBits:size_pos -> #cBits:size_pos ->
+  rBits:size_pos{nBits + 1 + rBits < max_size_t} ->
+  nInv_u64:bignum 64 -> n:bignum nBits{bn_v n > 0} ->
+  c:bignum cBits{nBits < rBits /\ cBits < nBits + rBits} ->
+  Tot (repeatable #(bignum (nBits + 1 + rBits)) #(rBits/64) (mont_pred #nBits #cBits rBits nInv_u64 n c))
+  #reset-options "--z3rlimit 150 --max_fuel 0"
 let mont_reduction_f #nBits #cBits rBits nInv_u64 n c i res =
   let res_i = bn_get_bits res (i * 64) ((i + 1)*64) in
   let qi = bn_get_bits (bn_mul nInv_u64 res_i) 0 64 in
-  let (c, res1) = bn_lshift_mul_add n (64*i) qi res in
-  assert (bn_v res1 + uint_v c * pow2 (nBits + 1 + rBits) == bn_v res + (bn_v n) * pow2 (64*i) * (bn_v qi));
-  assume (bn_v res + (bn_v n) * pow2 (64*i) * (bn_v qi) < pow2 (nBits + 1 + rBits));
-  assert (uint_v c == 0);
+  assert (bn_v qi <= pow2 64 - 1);
+  let (c1, res1) = bn_lshift_mul_add n (64*i) qi res in
+  assert (bn_v res1 + uint_v c1 * pow2 (nBits + 1 + rBits) == bn_v res + bn_v n * pow2 (64*i) * bn_v qi); //from bn_lshift_mul_add
+  assert (bn_v res + bn_v n * pow2 (64*i) * bn_v qi <= bn_v c + (pow2 (64*i)-1) * bn_v n + bn_v n * pow2 (64*i) * bn_v qi); //from ind hypo
+  assert (bn_v res + bn_v n * pow2 (64*i) * bn_v qi <= bn_v c + (pow2 (64*i)-1) * bn_v n + bn_v n * pow2 (64*i) * (pow2 64 - 1));
+  assert (bn_v res + bn_v n * pow2 (64*i) * bn_v qi <= bn_v c + pow2 (64*i) * bn_v n - bn_v n + bn_v n * pow2 (64*i) * (pow2 64 - 1));
+  assert (bn_v res + bn_v n * pow2 (64*i) * bn_v qi <= bn_v c + pow2 (64*i) * bn_v n - bn_v n + bn_v n * pow2 (64*i) * pow2 64 - bn_v n * pow2 (64*i));
+  assert (bn_v res + bn_v n * pow2 (64*i) * bn_v qi <= bn_v c - bn_v n + bn_v n * pow2 (64*i) * pow2 64);
+  assert (bn_v res + bn_v n * pow2 (64*i) * bn_v qi <= bn_v c + (pow2 (64*i) * pow2 64 - 1) * bn_v n);
+  pow2_plus (64*i) 64;
+  assert (64*(i+1) <= rBits);
+  assert (bn_v res + bn_v n * pow2 (64*i) * bn_v qi <= bn_v c + (pow2 (64*(i+1)) - 1) * bn_v n);
+  lemma_mont_reduction_f #nBits #cBits rBits n c i;
+  assert (bn_v res + bn_v n * pow2 (64*i) * bn_v qi < pow2 (nBits+rBits+1));
+  assert (bn_v res1 == bn_v res + pow2 (64*i) * bn_v qi * bn_v n);
+  lemma_mod_plus (bn_v res) (pow2 (64*i) * bn_v qi) (bn_v n); // res1 % n == res % n
   res1
 
 val mont_reduction_:
   #nBits:size_pos -> #cBits:size_pos ->
   rBits:size_pos{nBits < rBits /\ nBits + 1 + rBits < max_size_t /\ rBits % 64 == 0} ->
-  nInv_u64:bignum 64 -> n:bignum nBits ->
-  c:bignum cBits{cBits < nBits + 1 + rBits} ->
-  Tot (res:bignum (nBits + 1 + rBits))
+  nInv_u64:bignum 64 -> n:bignum nBits{bn_v n > 0} ->
+  c:bignum cBits{cBits < nBits + rBits} ->
+  Tot (res:bignum (nBits + 1 + rBits){bn_v res % bn_v n = bn_v c % bn_v n && bn_v res <= bn_v c + (pow2 rBits - 1) * bn_v n})
 
 let mont_reduction_ #nBits #cBits rBits nInv_u64 n c =
-  assume (bn_v c < pow2 (nBits + 1 + rBits));
-  let tmp = bn_cast_gt (nBits + 1 + rBits) c in
+  pow2_lt_compat (nBits+1+rBits) cBits;
+  let tmp = bn_cast_gt (nBits+1+rBits) c in
   let rLen = rBits / 64 in
-  repeati rLen
-  (fun i res ->
-    mont_reduction_f rBits nInv_u64 n c i res) tmp
+  let res = repeati_inductive rLen
+    (mont_pred #nBits #cBits rBits nInv_u64 n c)
+    (fun i res ->
+      mont_reduction_f rBits nInv_u64 n c i res) tmp in
+  res
 
 val mont_reduction:
   #nBits:size_pos -> #cBits:size_pos ->
   rBits:size_pos{nBits < rBits /\ nBits + 1 + rBits < max_size_t /\ rBits % 64 == 0} ->
-  nInv_u64:bignum 64 -> n:bignum nBits ->
-  c:bignum cBits{cBits < nBits + 1 + rBits} -> Tot (res:bignum (nBits+1))
+  nInv_u64:bignum 64 -> n:bignum nBits{bn_v n > 0} ->
+  c:bignum cBits{cBits < nBits + rBits} -> Tot (res:bignum (nBits+1){bn_v res % bn_v n == (bn_v c / pow2 rBits) % bn_v n})
 
 let mont_reduction #nBits #cBits rBits nInv_u64 n c =
   let tmp = mont_reduction_ rBits nInv_u64 n c in
+  assert (bn_v tmp % bn_v n = bn_v c % bn_v n && bn_v tmp <= bn_v c + (pow2 rBits - 1) * bn_v n);
+  lemma_mont_reduction #nBits #cBits rBits n c;
   let res = bn_rshift tmp rBits in
+  assert (bn_v res % bn_v n == (bn_v tmp / pow2 rBits) % bn_v n);
+  lemma_mod_mult_div_1 (bn_v tmp) (pow2 rBits) (bn_v n);
+  assert (bn_v res % bn_v n == ((bn_v c % bn_v n) / pow2 rBits) % bn_v n);
+  lemma_mod_mult_div_1 (bn_v c) (pow2 rBits) (bn_v n);
   res
 
 val mul_mod_mont:
   nBits:size_pos ->
-  rBits:size_pos{nBits + 1 < rBits /\ nBits + rBits + 1 < max_size_t /\ rBits % 64 == 0} ->
-  nInv_u64:bignum 64 -> n:bignum nBits ->
-  a:bignum (nBits+1) -> b:bignum (nBits+1) -> Tot (res:bignum (nBits+1))
+  rBits:size_pos{nBits + 2 < rBits /\ nBits + rBits + 1 < max_size_t /\ rBits % 64 == 0} ->
+  nInv_u64:bignum 64 -> n:bignum nBits{bn_v n > 0} ->
+  a:bignum (nBits+1) -> b:bignum (nBits+1) -> Tot (res:bignum (nBits+1){bn_v res % bn_v n == ((bn_v a * bn_v b) / pow2 rBits) % bn_v n})
 let mul_mod_mont nBits rBits nInv_u64 n a b =
   let c = bn_mul a b in
+  assert (bn_v c < pow2 (nBits + nBits + 2));
   mont_reduction rBits nInv_u64 n c
 
 val to_mont:
   #aBits:size_pos -> nBits:size_pos ->
   rBits:size_pos{nBits < rBits /\ nBits + rBits + 1 < max_size_t /\ rBits % 64 == 0} ->
-  nInv_u64:bignum 64 -> n:bignum nBits ->
-  r2:bignum nBits -> a:bignum aBits{aBits <= nBits} -> Tot (res:bignum (nBits+1))
+  nInv_u64:bignum 64 -> n:bignum nBits{bn_v n > 0} ->
+  r2:bignum nBits{bn_v r2 == pow2 (2*rBits) % bn_v n} ->
+  a:bignum aBits{aBits <= nBits} -> Tot (res:bignum (nBits+1){bn_v res % bn_v n == (bn_v a * pow2 rBits) % bn_v n})
+  #reset-options "--z3rlimit 50 --max_fuel 0"
 let to_mont #aBits nBits rBits nInv_u64 n r2 a =
   let c = bn_mul a r2 in
+  assert (bn_v c < pow2 (aBits + nBits));
   let res = mont_reduction rBits nInv_u64 n c in
+  assert (bn_v res % bn_v n == (bn_v c / pow2 rBits) % bn_v n);
+  lemma_mod_mult_div_1 (bn_v c) (pow2 rBits) (bn_v n);
+  assert (bn_v c % bn_v n == (bn_v a * bn_v r2) % bn_v n);
+  lemma_mod_mul_distr_l (bn_v r2) (bn_v a) (bn_v n);
+  lemma_mod_mul_distr_l (pow2 (2*rBits)) (bn_v a) (bn_v n);
+  lemma_mod_mult_div_1 (bn_v a * pow2 (2*rBits)) (pow2 rBits) (bn_v n);
+  assert (bn_v res % bn_v n == ((bn_v a * pow2 (2*rBits)) / pow2 rBits) % bn_v n);
+  pow2_multiplication_division_lemma_1 (bn_v a) rBits (2*rBits);
+  assert (bn_v res % bn_v n == (bn_v a * pow2 rBits) % bn_v n);
   res
 
 val from_mont:
   nBits:size_pos ->
   rBits:size_pos{nBits < rBits /\ nBits + rBits + 1 < max_size_t /\ rBits % 64 == 0} ->
-  nInv_u64:bignum 64 -> n:bignum nBits ->
-  a_r:bignum (nBits+1) -> Tot (res:bignum nBits)
-
+  nInv_u64:bignum 64 -> n:bignum nBits{bn_v n > 0} ->
+  a_r:bignum (nBits+1) -> Tot (res:bignum nBits{bn_v res == (bn_v a_r / pow2 rBits) % bn_v n})
+  #reset-options "--z3rlimit 50 --max_fuel 0"
 let from_mont nBits rBits nInv_u64 n a_r =
   let tmp = mont_reduction_ rBits nInv_u64 n a_r in
+  assert (bn_v tmp % bn_v n = bn_v a_r % bn_v n && bn_v tmp < bn_v a_r + pow2 rBits * bn_v n);
   let res = bn_rshift tmp rBits in
-  assume (bn_v res < pow2 nBits);
+  lemma_mod_mult_div_1 (bn_v tmp) (pow2 rBits) (bn_v n);
+  lemma_mod_mult_div_1 (bn_v a_r) (pow2 rBits) (bn_v n);
+  assume (bn_v res < bn_v n);
   let res = bn_cast_le nBits res in
+  small_modulo_lemma_1 (bn_v res) (bn_v n);
   res
+
+val mod_exp_pred:
+  nBits:size_pos ->
+  rBits:size_pos{nBits + 1 < rBits /\ nBits + rBits + 1 < max_size_t /\ rBits % 64 == 0} ->
+  nInv_u64:bignum 64 -> n:bignum nBits{bn_v n > 0} ->
+  bBits:size_pos -> b:bignum bBits ->
+  a0:bignum (nBits+1) -> acc0:bignum (nBits+1) ->
+  i:size_nat{i <= bBits} ->
+  a_acc:tuple2 (bignum (nBits+1)) (bignum (nBits+1)) -> Tot Type0
+let mod_exp_pred nBits rBits nInv_u64 n bBits b a0 acc0 i (a, acc) =
+  if i = 0 then
+    bn_v acc % bn_v n = bn_v acc0 % bn_v n
+  else
+    bn_v acc % bn_v n = ((pow (bn_v a0) (bn_v (bn_get_bits_first b i)) * bn_v acc0) / pow (pow2 rBits) (bn_v (bn_get_bits_first b i))) % bn_v n
+
+val mod_exp_f:
+  nBits:size_pos ->
+  rBits:size_pos{nBits + 2 < rBits /\ nBits + rBits + 1 < max_size_t /\ rBits % 64 == 0} ->
+  nInv_u64:bignum 64 -> n:bignum nBits{bn_v n > 0} ->
+  bBits:size_pos -> b:bignum bBits ->
+  a0:bignum (nBits+1) -> acc0:bignum (nBits+1) -> Tot (repeatable #(tuple2 (bignum (nBits+1)) (bignum (nBits+1))) #bBits (mod_exp_pred nBits rBits nInv_u64 n bBits b a0 acc0))
+  #reset-options "--z3rlimit 50 --max_fuel 0"
+let mod_exp_f nBits rBits nInv_u64 n bBits b a0 acc0 i (a, acc) =
+  let acc = if (bn_get_bit b i = 1) then mul_mod_mont nBits rBits nInv_u64 n a acc else acc in
+  let a = mul_mod_mont nBits rBits nInv_u64 n a a in
+  assume (mod_exp_pred nBits rBits nInv_u64 n bBits b a0 acc0 (i+1) (a, acc));
+  (a, acc)
 
 val mod_exp_:
   nBits:size_pos ->
-  rBits:size_pos{nBits + 1 < rBits /\ nBits + rBits + 1 < max_size_t /\ rBits % 64 == 0} ->
-  nInv_u64:bignum 64 -> n:bignum nBits ->
-  a:bignum (nBits+1) ->
+  rBits:size_pos{nBits + 2 < rBits /\ nBits + rBits + 1 < max_size_t /\ rBits % 64 == 0} ->
+  nInv_u64:bignum 64 -> n:bignum nBits{bn_v n > 0} ->
+  a0:bignum (nBits+1) ->
   bBits:size_pos -> b:bignum bBits ->
-  acc:bignum (nBits+1) -> Tot (res:bignum (nBits+1))
-let mod_exp_ nBits rBits nInv_u64 n a bBits b acc =
-  let (a, acc) =
-    repeati bBits
-    (fun i (a, acc) ->
-      let acc = if (bn_get_bit b i = 1) then mul_mod_mont nBits rBits nInv_u64 n a acc else acc in
-      let a = mul_mod_mont nBits rBits nInv_u64 n a a in
-      (a, acc)
-    ) (a, acc) in
+  acc0:bignum (nBits+1) -> Tot (res:bignum (nBits+1){bn_v res % bn_v n == ((pow (bn_v a0) (bn_v b)) * (bn_v acc0) / pow (pow2 rBits) (bn_v b)) % bn_v n})
+  #reset-options "--z3rlimit 50 --max_fuel 0"
+let mod_exp_ nBits rBits nInv_u64 n a0 bBits b acc0 =
+  let (a, acc) = repeati_inductive bBits
+    (mod_exp_pred nBits rBits nInv_u64 n bBits b a0 acc0)
+    (fun i (a, acc) -> mod_exp_f nBits rBits nInv_u64 n bBits b a0 acc0 i (a, acc))
+    (a0, acc0) in
+  assert (bn_v acc % bn_v n = ((pow (bn_v a0) (bn_v (bn_get_bits_first b bBits)) * bn_v acc0) / pow (pow2 rBits) (bn_v (bn_get_bits_first b bBits))) % bn_v n);
+  assert (bn_v (bn_get_bits_first b bBits) == bn_v b);
   acc
 
 val mod_exp:
   #aBits:size_pos ->
   nBits:size_pos{64 <= nBits /\ 2 * 64 * (blocks nBits 64 + 1) < max_size_t} ->
   n:bignum nBits{0 < bn_v n} -> a:bignum aBits{aBits <= nBits} ->
-  bBits:size_pos -> b:bignum bBits -> Tot (res:bignum nBits)
+  bBits:size_pos -> b:bignum bBits -> Tot (res:bignum nBits{bn_v res == (pow (bn_v a) (bn_v b)) % bn_v n})
 let mod_exp #aBits nBits n a bBits b =
   let nLen = blocks nBits 64 in
   let rBits = 64 * (nLen + 1) in
@@ -130,8 +201,12 @@ let mod_exp #aBits nBits n a bBits b =
   let n0 = bn_get_bits n 0 64 in
   let nInv_u64 = bn_from_u64 (mod_inv_u64 (bn_to_u64 n0)) in
   let a_r = to_mont nBits rBits nInv_u64 n r2 a in
+  assert (bn_v a_r % bn_v n == (bn_v a * pow2 rBits) % bn_v n);
   let acc_r = to_mont nBits rBits nInv_u64 n r2 (bn_const_1 #nBits) in
+  assert (bn_v acc_r % bn_v n == pow2 rBits % bn_v n);
   let res_r = mod_exp_ nBits rBits nInv_u64 n a_r bBits b acc_r in
+  assert (bn_v res_r % bn_v n == ((pow (bn_v a_r) (bn_v b)) * (bn_v acc_r) / pow (pow2 rBits) (bn_v b)) % bn_v n);
+  admit();
   let res = from_mont nBits rBits nInv_u64 n res_r in
   res
 
@@ -142,7 +217,7 @@ val rsa_blinding:
   qBits:size_pos{pBits + qBits + 64 < max_size_t} -> q:bignum qBits{0 < bn_v q /\ bn_v n == bn_v p * bn_v q} ->
   m:bignum mBits{mBits <= nBits} ->
   dBits:size_pos{dBits < pBits + qBits + 64} -> d:bignum dBits ->
-  rBlind:bignum 64 -> Tot (s:bignum nBits)
+  rBlind:bignum 64 -> Tot (s:bignum nBits{bn_v s == (pow (bn_v m) (bn_v d)) % bn_v n})
 let rsa_blinding #mBits nBits n pBits p qBits q m dBits d rBlind =
   let bn_1 = bn_const_1 #1 in
   let p1 = bn_sub p bn_1 in
@@ -154,4 +229,5 @@ let rsa_blinding #mBits nBits n pBits p qBits q m dBits d rBlind =
   assume (bn_v d1 + bn_v d < pow2 (pBits + qBits + 64));
   assert (uint_v c == 0);
   let s = mod_exp nBits n m (pBits + qBits + 64) d2 in
+  admit();
   s
